@prefix rdf: <http://www.w3.org/1999/02/22-rdf-syntax-ns#> .
@prefix owl: <http://www.w3.org/2002/07/owl#> .
@prefix dc: <http://purl.org/dc/elements/1.1/> .
@prefix xsd: <http://www.w3.org/2001/XMLSchema#> .
@prefix vann: <http://purl.org/vocab/vann/> .
@prefix foaf: <http://xmlns.com/foaf/0.1/> .
@prefix usdl: <http://www.linked-usdl.org/ns/usdl#> .
@prefix rdfs: <http://www.w3.org/2000/01/rdf-schema#> .
@prefix gr: <http://purl.org/goodrelations/v1#> .
@prefix skos: <http://www.w3.org/2004/02/skos/core#> .
@prefix org: <http://www.w3.org/ns/org#> .


<http://linked-usdl.org/ns/usdl> a owl:Ontology;
    dc:title "Linked-USDL Core";
    dc:description """<p>This vocabulary provides the core module of Linked USDL. It therefore covers the main concepts and properties characterising services, leaving more specific aspects regarding some particular dimensions such as technical interfaces, licensing or security aside. These aspects will be covered in additional modules, or &nbsp;in some cases, like the technical interfaces, by existing vocabularies.</p>
<p>This first draft includes most of the original USDL specification with some useful simplifications. </p>
""";
    dc:modified "2012-09-20"^^xsd:date;
    vann:preferredNamespaceUri "http://www.linked-usdl.org/ns/usdl#";
    vann:preferredNamespacePrefix "usdl";
    foaf:page <http://linked-usdl.org/ns/usdl.html>;
    dc:creator
        <http://linked-usdl.org/ns/usdl#cpedrinaci>,
        <http://linked-usdl.org/ns/usdl#jcardoso>,
        <http://linked-usdl.org/ns/usdl#tleidig> .

<http://linked-usdl.org/ns/usdl#cpedrinaci> a foaf:Person;
    foaf:name "Carlos Pedrinaci";
    foaf:homepage <http://www.cpedrinaci.net> .

<http://linked-usdl.org/ns/usdl#jcardoso> a foaf:Person;
    foaf:name "Jorge Cardoso";
    foaf:homepage <http://eden.dei.uc.pt/~jcardoso/> .

<http://linked-usdl.org/ns/usdl#CISUC%2C%20University%20of%20Coimbra> a foaf:Organization;
    foaf:member <http://linked-usdl.org/ns/usdl#jcardoso>;
    foaf:name "CISUC/DEI, University of Coimbra";
    foaf:homepage <http://www.dei.uc.pt> .

<http://linked-usdl.org/ns/usdl#Knowledge%20Media%20Institute%2C%20The%20Open%20University> a foaf:Organization;
    foaf:member <http://linked-usdl.org/ns/usdl#cpedrinaci>;
    foaf:name "Knowledge Media Institute, The Open University";
    foaf:homepage <http://www.open.ac.uk> .

<http://linked-usdl.org/ns/usdl#tleidig> a foaf:Person;
    foaf:name "Torsten Leidig".

<http://linked-usdl.org/ns/usdl#SAP%20Research%20Center%20CEC%20Karlsruhe%2C%20SAP%20AG> a foaf:Organization;
    foaf:member <http://linked-usdl.org/ns/usdl#tleidig>;
    foaf:name "SAP Research Center CEC Karlsruhe, SAP AG";
    foaf:homepage <http://www.sap.com> .

usdl:Service a rdfs:Class, owl:Class;
    rdfs:isDefinedBy <http://linked-usdl.org/ns/usdl>;
    rdfs:label "service";
    rdfs:comment "A usdl:Service is a 'black box' description of a service for the purpose of describing the service in a way that it can serve as an interface between the provider and the consumer. The description contains functional properties of the service, described by the interaction protocol as well as non-functional properties described by qualitative or quantitative values. Any composite implementation of a service that is internal is invisible, however arbitrarily complex an actual service composition may be, it can be described using supplemental service network vocabularies, which are beyond the USDL Core vocabulary.";
    rdfs:subClassOf gr:ProductOrService .

usdl:ServiceOffering a rdfs:Class, owl:Class;
    rdfs:isDefinedBy <http://linked-usdl.org/ns/usdl>;
    rdfs:label "service offering";
    rdfs:comment "A service offering is an offering made by a gr:BusinessEntity of one or more services to the public or specific customers. It  usually gives defines a price and terms and conditions including service level agreements";
    rdfs:subClassOf gr:Offering .

usdl:Parameter a rdfs:Class, owl:Class;
    rdfs:isDefinedBy <http://linked-usdl.org/ns/usdl>;
    rdfs:label "parameter";
    rdfs:comment "Parameter is used to capture conceptual input to and output of interactions. Parameters, on the one hand, may be something very vague, like an idea. On the other hand, they can be something specific, such as the architecture blueprint of a building." .

usdl:InteractionPoint a rdfs:Class, owl:Class;
    rdfs:isDefinedBy <http://linked-usdl.org/ns/usdl>;
    rdfs:label "Represetn an interaction point";
    rdfs:comment "An InteractionPoint represents an actual step in accessing and performing operations of the service. On a technical level this could translate into calling a Web Service operation. On a professional level, it could mean that consumer and provider meet in person to exchange service parameters or resources involved in the service delivery (e.g. documents that are processed by the provider). An interaction can be initiated by the consumer or the provider." .

usdl:ServiceModel a rdfs:Class, owl:Class;
    rdfs:isDefinedBy <http://linked-usdl.org/ns/usdl>;
    rdfs:label "service model";
    rdfs:comment "A ServiceModel is used to represent 'classes' of services, i.e. services that share a number of characteristics.  ServiceModel enables the capturing of these characteristics.";
    rdfs:subClassOf
        usdl:Service,
        gr:ProductOrServiceModel .

usdl:Condition a rdfs:Class, owl:Class;
    rdfs:isDefinedBy <http://linked-usdl.org/ns/usdl>;
    rdfs:label "Condition";
    rdfs:comment """<p>The class of conditions for a milstone. Preconditions or postcondition</p>""". 

usdl:hasServiceModel a rdf:Property;
    rdfs:isDefinedBy <http://linked-usdl.org/ns/usdl>;
    rdfs:label "has service model";
    rdfs:comment "Refers to the service model that specifies properties valid for all services of this model";
    rdfs:domain usdl:Service;
    rdfs:range usdl:ServiceModel;
    rdfs:subPropertyOf gr:hasMakeAndModel .

usdl:hasClassification a rdf:Property;
    rdfs:subPropertyOf dc:subject;
    rdfs:isDefinedBy <http://linked-usdl.org/ns/usdl>;
    rdfs:label "classification";
    rdfs:comment "Indicates a classification of a service.";
    rdfs:domain usdl:Service;
    rdfs:range skos:Concept.

usdl:hasPrecondition a rdf:Property;
    rdfs:isDefinedBy <http://linked-usdl.org/ns/usdl>;
    rdfs:label "has precondition";
    rdfs:comment """<p>Preconditions to be fulfilled to perform the Interaction or InteractionProtocol.</p>""";
    rdfs:domain usdl:Interaction;
    rdfs:range usdl:Condition .

usdl:hasInteractionPoint a rdf:Property;
    rdfs:isDefinedBy <http://linked-usdl.org/ns/usdl>;
    rdfs:label "has interaction";
    rdfs:comment """<p>Interactions that are part of the interaction protocol</p>""";
    rdfs:domain usdl:Service;
    rdfs:range usdl:InteractionPoint .

usdl:hasInput a rdf:Property;
    rdfs:isDefinedBy <http://linked-usdl.org/ns/usdl>;
    rdfs:label "has input";
    rdfs:comment """<p>Input parameters required for the interaction</p>""";
    rdfs:domain usdl:InteractionPoint;
    rdfs:range usdl:Parameter;
    rdfs:subPropertyOf usdl:hasParameter .

usdl:hasPostcondition a rdf:Property;
    rdfs:isDefinedBy <http://linked-usdl.org/ns/usdl>;
    rdfs:label "has postcondition";
    rdfs:comment """<p>Postcondition that holds if the phase was performed successfully</p>""";
    rdfs:domain usdl:InteractionPoint;
    rdfs:range usdl:Condition .


usdl:includes a rdf:Property;
    rdfs:isDefinedBy <http://linked-usdl.org/ns/usdl>;
    rdfs:label "includes";
    rdfs:comment """A ServiceOffering bundles a number of services and associates concrete service levels and pricing for for the purpose of selling to customers. The ServiceOffering is the client's view on services on a service marketplace. Services are usually purchased via a specific ServiceOffering.""";
    rdfs:subPropertyOf gr:includes;
    rdfs:domain usdl:ServiceOffering;
    rdfs:range usdl:Service .

usdl:hasInteractionPoint a rdf:Property;
    rdfs:isDefinedBy <http://linked-usdl.org/ns/usdl>;
    rdfs:label "has interaction point";
    rdfs:comment "Interaction point is a logical point were a consumer interacts with a supplier.";
    rdfs:domain usdl:Service;
    rdfs:range usdl:InteractionPoint .

usdl:hasParameter a rdf:Property;
    rdfs:isDefinedBy <http://linked-usdl.org/ns/usdl>;
    rdfs:label "has parameter";
    rdfs:comment """<p>Input parameters required for the interaction</p>""";
    rdfs:domain usdl:InteractionPoint;
    rdfs:range usdl:Parameter .

usdl:hasOutput a rdf:Property;
    rdfs:isDefinedBy <http://linked-usdl.org/ns/usdl>;
    rdfs:label "has output";
    rdfs:comment """<p>Output parameters required for the function</p>""";
    rdfs:domain usdl:InteractionPoint;
    rdfs:range usdl:Parameter;
    rdfs:subPropertyOf usdl:hasParameter .

usdl:hasInteractionType a rdf:Property;
    rdfs:isDefinedBy <http://linked-usdl.org/ns/usdl>;
    rdfs:label "has interaction type";
    rdfs:comment "How can a customer participate in an interaction.
                  Possible values are: Human-Machine, Human-Human, Machine-Human, Machine-Machine";
    rdfs:domain usdl:InteractionPoint;
    rdfs:range <http://www.w3.org/2000/01/rdf-schema#Literal>.

usdl:hasInteractionSpace a rdf:Property;
    rdfs:isDefinedBy <http://linked-usdl.org/ns/usdl>;
    rdfs:label "has interaction space";
    rdfs:comment "Does the interaction between customer and provider occurs at the same physical place? 
                  Or the interaction is mediated by technology?
                  Possible values are: Presential, Remote";
    rdfs:domain usdl:InteractionPoint;
    rdfs:range <http://www.w3.org/2000/01/rdf-schema#Literal>.


usdl:hasParticipant a rdf:Property;
    rdfs:isDefinedBy <http://linked-usdl.org/ns/usdl>;
    rdfs:label "has participant";
    rdfs:comment "Captures the participants involved in a concrete Interaction.";
    rdfs:domain usdl:InteractionPoint;
    rdfs:range usdl:Participant.

usdl:Participant a rdfs:Class, owl:Class;
    rdfs:isDefinedBy <http://linked-usdl.org/ns/usdl>;
    rdfs:label "Participant";
    rdfs:comment "Participant is a class to capture the participation of Entities in a certain Interaction".

usdl:hasAgent a rdf:Property;
    rdfs:isDefinedBy <http://linked-usdl.org/ns/usdl>;
    rdfs:label "has agent";
    rdfs:comment "Captures the participants involved in a concrete Interaction.";
    rdfs:domain usdl:Participant;
    rdfs:range gr:BusinessEntity.

usdl:hasRole a rdf:Property;
    rdfs:isDefinedBy <http://linked-usdl.org/ns/usdl>;
    rdfs:label "has role";
    rdfs:comment "Role played in a particular Interaction.";
    rdfs:domain usdl:Participant;
    rdfs:range usdl:Role.

usdl:Role a skos:Concept;
    rdfs:isDefinedBy <http://linked-usdl.org/ns/usdl>;
    rdfs:label "Types of Roles";
    rdfs:comment "The kinds of Role that an entity may play within a certain Interaction".

# some important roles

usdl:Provider a usdl:Role;
    rdfs:label "Provider";
    skos:prefLabel "Provider";
    skos:altLabel "Supplier";
    skos:definition "A Provider is the entity responsible for providing the Service".

usdl:Consumer a usdl:Role;
    rdfs:label "Consumer";
    skos:prefLabel "Consumer";
    skos:definition "A Consumer is the entity actually using the Service".

usdl:Partner a usdl:Role;
    rdfs:label " Partner";
    skos:prefLabel "Partner";
    skos:definition "An business partner is any other participant that acts on behalf of the provider as a third party".

